

1

- Algebras, modules, and functors

~ I. Rings and algebras

Defⁿ: A ring is an additive group R with bilinear (mult) oper $\cdot: R \times R \rightarrow R$ and unit $1 \in R$ for which

$$(a \cdot b) \cdot c = a \cdot (b \cdot c) \quad \text{and} \quad 1 \cdot a = a = a \cdot 1$$

at all a, b, c in R .

Note that bilinearity gives

$$\begin{cases} a \cdot (b + b') = ab + ab' \\ (a + a') \cdot b = ab + a'b \end{cases}$$

We call a ring R commutative if $a \cdot b = b \cdot a$ for all a, b in R .

Defⁿ: A ring homomorphism/map is an additive group map $f: R \rightarrow S$ for which
 $f(a \cdot b) = f(a) \cdot f(b)$ at all a, b in R and
 $f(1_R) = 1_S$.

Defⁿ: For a ring R the opposite ring R^{op} is the same additive group w/ multiplication $a \cdot_{\text{op}} b := b \cdot a$ and unit $1_{R^{\text{op}}} = 1_R$.

Defⁿ: The center of a ring $Z(R)$ is the collection of all $a \in R$ for which $a \cdot b = b \cdot a$ at all b in R . We call a ring map $f: S \rightarrow R$

from a commutative ring S central if $f(S) \subseteq Z(R)$.

Def^t: For a fixed commutative ring k , a k -algebra R is a ring R equipped with a central ring map $\text{unit}_R: k \rightarrow R$. A map of k -algebras $f: R \rightarrow S$ is a ring map for which the diagram

$$\begin{array}{ccc} R & \xrightarrow{f} & S \\ \text{unit}_R \swarrow & k & \searrow \text{unit}_S \end{array}$$

commutes.

~ § 1/3 Ideals and quotient rings.

Def^t: An ideal $I \subseteq A$ in a ring A is an additive subgroup I which
 $a \cdot m$ and $m \cdot a \in I$ whenever $m \in I, a \in A$.

Lemma 1: For any ideal $I \subseteq A$ the additive quotient A/I inherits a unique ring structure under which the quotient map $\pi: A \rightarrow A/I$ is a ring map. Furthermore, for any ring map $\phi: A \rightarrow B$ with $I \subseteq \ker(\phi)$, there is a unique ring map $\bar{\phi}: A/I \rightarrow B$

which completes the diagram

$$\begin{array}{ccc} A & \xrightarrow{\varphi} & B \\ \pi \downarrow & & \uparrow \bar{\varphi} \\ A/I & \xrightarrow{\bar{\varphi}} & B \end{array}$$

3

Construction/Proof: For $\bar{a} = a + I$ in A/I

we claim that the product

$$\bar{a} \cdot \bar{b} := \overline{a \cdot b} \quad \text{is well defined, i.e. independent}$$

of choice of reps a and b in A . This is clear

since I is stable under the action of A on the right

and left. The unit in A/I is $1_{A/I} = \bar{1}_A$.

For $\bar{\varphi} : A/I \rightarrow B$, we have

such a unique map of additive groups, and for $\bar{a}, \bar{b} \in A/I$

we check the product $\bar{\varphi}(\bar{a} \cdot \bar{b}) = \bar{\varphi}(\overline{a \cdot b}) = \bar{\varphi}(\pi(ab))$

$$= \bar{\varphi}(ab) = \varphi(a) \cdot \varphi(b) = \bar{\varphi}(\bar{a}) \cdot \bar{\varphi}(\bar{b})$$

and also $\bar{\varphi}(\bar{1}) = \bar{\varphi}(1) = 1$. So $\bar{\varphi}$ is a ring map.

Lemma 2: The kernel of any ring map $\varphi : A \rightarrow B$ is an ideal $\ker(\varphi) \subseteq A$.

Def¹: For elements $a_1, \dots, a_n \in A$ the ideal generated by a_1, \dots, a_n is the smallest ideal in A which contains the given elements, i.e. the intersection $\subseteq \Sigma$

$$(a_1, \dots, a_n) = \bigcap_{I \in \Sigma} I \quad \text{over the set of ideals } I \text{ w/ } (a_i \in I).$$

Lemma 3: For any collection of elements $a_1, \dots, a_n \in A$ we have

$$(a_1, \dots, a_n) = \sum_{i=1}^n A \cdot a_i \cdot A = \left\{ \sum_{i=1}^n b_i a_i b'_i : b_i, b'_i \in A \right\}.$$

When A is commutative

$$(a_1, \dots, a_n) = \sum_{i=1}^n A \cdot a_i = \left\{ \sum_{i=1}^n b_i a_i : b_i \in A \right\}.$$

Example: For any field K , all ideals in $K[X]$ are of the form $(p) \subseteq K[X]$, for p a polynomial in $K[X]$, and $(p) = \{ g \in K[X] : p \text{ divides } g \}$.
This follows by the division algorithm.

Example [HW]: For any field K , the only ideals I in $M_n(K)$ are $\{0\}$, and $M_n(K)$ itself.

~ 1 2/3 Product of rings

For any collection of rings A_λ , indexed by a set Λ , the additive product $\prod_{\lambda \in \Lambda} A_\lambda$ admits a ring structure w/ product

$$(a_\lambda : \lambda \in \Lambda) \cdot (b_\lambda : \lambda \in \Lambda) = (a_\lambda \cdot b_\lambda : \lambda \in \Lambda)$$

and unit $1 = (1_{A_\lambda} : \lambda \in \Lambda)$.

Note that we have ring maps

$p_\lambda: \prod_{\lambda \in \Lambda} A_\lambda \rightarrow A_\lambda$, $p_\lambda(a_\lambda, \lambda \in \Lambda) = a_\lambda$
at each λ in Λ .

Exercise: Any collection of ring maps $\phi_\lambda: A \rightarrow A_\lambda$,
across all λ in Λ , determines a unique ring map
 $\phi: A \rightarrow \prod_{\lambda \in \Lambda} A_\lambda$ for which $p_\lambda \circ \phi = \phi_\lambda$ at
each λ in Λ .

Question: Is the inclusion $\iota_0: A \rightarrow A \times A$,
 $\iota_0(a) = (a, 0)$, a ring map?

~ II. Categories and functors

A category is a class of objects $\text{obj } \mathcal{C}$ which
is paired w/ a set of morphisms $\text{Hom}_{\mathcal{C}}(x, y)$ at each
 x, y in \mathcal{C} and associative composition operations

$$\circ: \text{Hom}_{\mathcal{C}}(x_1, x_2) \times \text{Hom}_{\mathcal{C}}(x_0, x_1) \rightarrow \text{Hom}_{\mathcal{C}}(x_0, x_2)$$

We also require the specification of identity morphisms
 $\text{id}_x: x \rightarrow x$ at each x in \mathcal{C} for which
 $f \circ \text{id}_x = f = \text{id}_y \circ f$ at each $f \in \text{Hom}_{\mathcal{C}}(x, y)$.

A functor between categories $F: \mathcal{C} \rightarrow \mathcal{D}$

α a choice of set map $\text{obj}(F): \text{obj}(\mathcal{C}) \rightarrow \text{obj}(\mathcal{D})$

and, for each x, y in \mathcal{C} , a set map

$$F_{xy}: \text{Hom}_{\mathcal{C}}(x, y) \rightarrow \text{Hom}_{\mathcal{D}}(F(x), F(y))$$

for which

$$F(g \circ f) = F(g) \circ F(f)$$

at each sequence $x \xrightarrow{f} y \xrightarrow{g} z$ in \mathcal{C} .

Remark: Obs. we've abused notation to take $F = \text{obj}(F)$ and/or $F = F_{xy}$ when convenient.

Defⁿ: For $F, F': \mathcal{C} \rightarrow \mathcal{D}$ functors, a natural transformation $\xi: F \rightarrow F'$ is a collection of

maps $\xi_x: F(x) \rightarrow F'(x)$ in \mathcal{D} , at each x in \mathcal{C} , for which the diagram


$$\begin{array}{ccc} F(x) & \xrightarrow{\xi_x} & F'(x) \\ F(f) \downarrow & & \downarrow F'(f) \\ F(y) & \xrightarrow{\xi_y} & F'(y) \end{array} \quad \text{commutes, at each } f \text{ in } \mathcal{C}.$$

Note that we can compose natural transformations, in the apparent way, so that we have a category $\text{Fun}(\mathcal{C}, \mathcal{D})$ of functors and transformations

Defⁿ: A morphism $f: x \rightarrow y$ in a category \mathcal{C} is called an isomorphism if there exists $g: y \rightarrow x$

for which $g \circ f = id_x$ and $f \circ g = id_y$.

Lemma 4: A natural transformation $\xi: F \rightarrow F'$ between functors is a natural isomorphism, i.e. an isom in the cat $\text{Fun}(C, D)$, if and only if each $\xi_x: F(x) \rightarrow F'(x)$ is an isomorphism in D .

Proof: Exercise. 

Def¹: A functor $F: C \rightarrow D$ is said to be an equivalence of categories if there exists some functor $G: D \rightarrow C$ and natural isomorphism

$$\xi: G \circ F \xrightarrow{\sim} id_C, \quad \xi': F \circ G \xrightarrow{\sim} id_D.$$

I will call a functor $F: C \rightarrow D$ an isomorphism of categories if there exists $G: D \rightarrow C$ for which $G \circ F = id_C$ and $F \circ G = id_D$.


Def²: Given a functor $F: C \rightarrow D$ w/ maps in $\text{Hom}_C(x, y) \rightarrow \text{Hom}_D(Fx, Fy)$, we call F

i) Faithful if each map F_{xy} is injective.

ii) Fully faithful if each F_{xy} is bijective.

iii) Essentially surjective if each x in D admits an x in C for which there is an isomorphism $x \xrightarrow{\sim} F(x)$ in D .

Theorem 5: A functor $F: C \rightarrow D$ is an equivalence if and only if F is fully faithful and essentially surjective.

Proof: Exercise. 

Defⁿ: For any category C the opposite category C^{op} has the same objects and morphisms as C , but the opposite composition

$$f \circ g := g \circ f.$$

Ex: We have the cat Ab of abelian groups and group homomorphisms, the cat $Ring$ of rings and ring homomorphisms, the cat Alg_K of K -algs and K -alg homomorphisms, the cat Set of sets and set maps, the cat $Field_F$ of field extensions of a given field F and maps over F , etc.

Ex: We have the fully faithful inclusion
 $\text{Fields}_{\mathbb{F}} \rightarrow \text{Alg}_{\mathbb{F}}, \begin{cases} K \mapsto K \\ f \mapsto f \end{cases}$

Ex: We have the free alg functor
 $\text{Free}_{\mathbb{F}}: \text{Set} \rightarrow \text{Alg}_{\mathbb{F}},$
 $X \mapsto \mathbb{C}[x: x \in X], \tau \mapsto (p(x) \mapsto p(\tau(x))).$

Ex: For any category \mathcal{C} , we have the functor


$Y_{\mathcal{C}}: \mathcal{C} \rightarrow \text{Fun}(\mathcal{C}^{\text{op}}, \text{Set})$
 $Y_{\mathcal{C}}(x) = \text{Hom}_{\mathcal{C}}(-, x), Y_{\mathcal{C}}(f) = f_{*-}$

Ex: For any comm ring K , we have the forgetful functor
 $\text{forget}: \text{Alg}_K \rightarrow \text{Ring}, \begin{cases} A \mapsto A \\ f \mapsto f \end{cases}$

Proposition 6: The forgetful functor

$\text{forget}: \text{Alg}_{\mathbb{Z}} \rightarrow \text{Ring}$

is an equivalence. In fact, it is an isomorphism.

Construction: The inverse $\text{alg}: \text{Ring} \rightarrow \text{Alg}_{\mathbb{Z}}$ takes a ring R to R equipped with the (unique) central ring map $\text{unit}_R: \mathbb{Z} \rightarrow R, n \mapsto n \cdot 1_R$. 

~ III. Modules and restriction

Let A be a ring. An A -module is an additive group M equipped with a bilinear map

$$\cdot : A \times M \rightarrow M$$

wt $a \cdot (b \cdot m) = (a \cdot b) \cdot m$ and $1 \cdot m = m$ at all a, b in A and m in M . A homomorphism of A -modules is an additive group map $f: M \rightarrow N$ so that $f(a \cdot m) = a \cdot f(m)$ at all a in A and m in M . A -mod

Def¹: The category of A -modules is the collection of all A -modules, with A -module homomorphisms.

Now, for any ring map $\phi: A \rightarrow B$ we have the restriction functor

$$\text{res} = \text{res}_\phi : B\text{-mod} \rightarrow A\text{-mod}$$

which sends a B -module N to N itself equipped

wt the action $a \cdot_\phi n := \phi(a) \cdot n$. Via the

$$\text{eg } f(a \cdot_\phi n) = f(\phi(a) \cdot n) = \phi(a) \cdot f(n) = a \cdot_\phi f(n),$$

we see that any B -module map $f: N \rightarrow N'$ becomes an A -module map $f: \text{res}_\phi(N) \rightarrow \text{res}_\phi(N')$, and so we can define res_ϕ explicitly on obj and morph by

$$\text{res}_\phi : \begin{cases} N \mapsto \text{res}_\phi(N) \\ f \mapsto f \end{cases} \quad //$$

Example: We have the ring map $x_1 \mapsto y_1^2$
 $\mathbb{C}[x_1, x_2, x_3] \rightarrow \mathbb{C}[y_1, y_2], \quad x_2 \mapsto y_2^2$
 $(x_1 x_2 - x_3^2) \quad x_3 \mapsto y_1 y_2$

so that any $\mathbb{C}[y_1, y_2]$ -module restricts to a module over $\mathbb{C}[x_1, x_2, x_3] / (x_1 x_2 - x_3^2)$.

Observation 7: For any k -algebra A , we have the restriction functor $A\text{-mod} \rightarrow k\text{-mod}$. In particular, when k is a field, any A -module is naturally a vector space, and any A -module map is naturally a vector space map over k , and any A -algebra map is a map of vector spaces over k .

~ IV. The abelian structure on $A\text{-mod}$ at all M

We have the zero module 0 w/ $\text{Hom}_A(M, 0) = 0 = \text{Hom}_A(0, M)$.

A submodule $M' \subseteq M$ is an A -module M' is an abelian subgroup for which $a \cdot m \in M'$ whenever m is in M' , and $a \in A$. We note that in this case M' itself is an A -module and the inclusion

$$\iota: M' \rightarrow M$$

is a map between A -modules.

Furthermore, for any submodule $M' \subseteq M$

The additive quotient M/M' inherits a unique A -module structure under which the quotient

$$(*) \quad \pi: M \rightarrow M/M', \quad m \mapsto \pi(m) = \bar{m},$$

is an A -module map. Explicitly,

$$a \cdot \bar{m} := \overline{a \cdot m}.$$

The projection $(*)$ is universal amongst A -module maps $f: M \rightarrow N$ for which $f|_{M'} = 0$.

(ii) Image is submodule

Lemma 8: i) For any A -module hom $f: M \rightarrow N$, the kernel $\ker(f) \subseteq M$ is an A -submodule.

ii) For any two maps $f, f': M \rightarrow N$, and central elements $z, z' \in Z(A)$ the linear combo $(zf + z'f'): m \mapsto z f(m) + z' f'(m)$ is also a map of A -modules.

iii) The zero map $0: M \rightarrow N$ is always an A -module map.

Proof: (i) For m in $\ker(f)$ and a in A we have $f(am) = af(m) = a \cdot 0 = 0$. Since the kernel is known to be an additive subgroup, we have that $\ker(f)$ is a submodule. (ii) Additivity is clear. For A -linearity we just check

$$\underbrace{(zf + z'f')(a \cdot m)}_{\text{central}} = z(a f(m)) + z'(a f'(m)) = a \cdot (zf(m) + z'f'(m)) = a \cdot ((zf + z'f')(m)).$$

Corollary 9: For any K -algebra A , and A -modules U and V , the set of A -module maps $\text{Hom}_A(U, V)$

is naturally a K -module.

Example: For $A = \mathbb{Q}[x]$, $U = \mathbb{Q}[x]/(x^2)$, $\text{Hom}_A(A, U)$ is 2-dimensional w/ basis spanned by the maps $\pi_0: A \rightarrow U$, $\pi_0(a) = \bar{a}$ and $\pi_1: A \rightarrow U$, $\pi_1(a) = \bar{a} \cdot \bar{x}$.

Example: For any field K we have the matrix algebra $M_n(K) = \text{End}_K(K^n)$ and the "standard module" $V = K^n$ with action $A \cdot v$ given by matrix action.

Then $\text{End}_{M_n(K)}(V)$ is 1-dimensional and spanned by the identity. This follows by considering eigenvectors for the action of the diagonal matrices, in conj w/ the action of the superdiagonals [HW].

Def^{1.5}: Call an A -module M simple (aka irreducible) if any submodule $M' \leq M$ is either zero, or equal to M .

Question: We have the field inclusion $\mathbb{R} \rightarrow \mathbb{C}$ under which \mathbb{C} becomes an \mathbb{R} -module. Is \mathbb{C} simple over \mathbb{R} ?

AW: Classify simple modules over $\mathbb{Q}[x]$.

Example: Any ideal $I \subseteq A$ is an A -submodule in A .

For the poly ring $K[x]$ over a field, all ideals $I \subseteq K[x]$ are isomorphic as modules. Indeed, for $I = (p)$ we have the module isomorphism

$$f_p: K[x] \xrightarrow{\cong} (p), \quad a \mapsto a \cdot p.$$

For injectivity ..., for surjectivity ...

~ IV 1/3 Generating submodules

For any A -module M and subset $X \subseteq M$ we have the submodule $A \cdot X \subseteq M$ generated by X . This submodule can be defined, for example, as the intersection of all submodules which contain X .

Lemma 10: For any subset $X \subseteq M$, the submodule gen'd by X in M is explicitly the subset $A \cdot X = \left\{ \sum_{i=1}^n a_i \cdot x_i : n \geq 0, a_i \in A, x_i \in X \right\} \subseteq M$.

~ IV $\frac{2}{3}$ Sum of modules

Given a collection of A -modules M_λ , indexed by a set Λ , the product module $\prod_{\lambda \in \Lambda} M_\lambda$ is the product of the additive groups, along with the A -action $a \cdot (m_\lambda : \lambda \in \Lambda) := (a \cdot m_\lambda : \lambda \in \Lambda)$.

The direct sum $\bigoplus_{\lambda \in \Lambda} M_\lambda$ is the submodule in $\prod_{\lambda \in \Lambda} M_\lambda$ consisting of all tuples $(m_\lambda : \lambda \in \Lambda)$ in which all but finitely many of the m_λ are 0.

When all of the $M_\lambda = A$, the regular A -mod, we call the sum $\bigoplus_{\lambda \in \Lambda} A$ the free module for A on the basis Λ . For such a free module we take I_λ the tuple with 1 in the λ -th position and 0 elsewhere. We have the set inclusion

$$(*) \quad i: \Lambda \rightarrow \bigoplus_{\lambda \in \Lambda} A, \quad i(\lambda) := I_\lambda.$$

Lemma 11: For any set Λ , and any A -module M , restriction along the inclusion $(*)$ provides a bijection of sets

$$i^*: \text{Hom}_{A\text{-mod}}\left(\bigoplus_{\lambda \in \Lambda} A, M\right) \xrightarrow{\cong} \text{Hom}_{\text{set}}(\Lambda, M).$$

Proof: For the inverse, take any set map $\xi: \Lambda \rightarrow M$ to the module homomorphism $\tilde{\xi}: \bigoplus_{\lambda \in \Lambda} A \rightarrow M$

defined by $\tilde{\Sigma}(\sum_{\lambda \in \Lambda} a_{\lambda} 1_{\lambda}) = \sum_{\lambda} a_{\lambda} \tilde{\Sigma}(\lambda)$,
 where only finitely many of the a_{λ} here are necessarily 0.

The fact that $\tilde{\Sigma}$ is additive is clear, and Λ -linearity is also clear. So $\tilde{\Sigma}$ is an Λ -module map. Furthermore $\tilde{\gamma}^*(\tilde{\Sigma}) = \tilde{\Sigma}|_{\Lambda} = \Sigma$ by construction.

Conversely, for an Λ -mod map $f: \bigoplus_{\lambda \in \Lambda} \Lambda \rightarrow M$ we have $(\tilde{\gamma}^*(f) - f)(1_{\lambda}) = f(1_{\lambda}) - f(1_{\lambda}) = 0$ at all $\lambda \in \Lambda$ which gives $(\tilde{\gamma}^*(f) - f)(\sum_{\lambda \in \Lambda} a_{\lambda} 1_{\lambda}) = 0$ at all $\sum_{\lambda \in \Lambda} a_{\lambda} 1_{\lambda}$ in $\bigoplus_{\lambda \in \Lambda} \Lambda$. Hence $\tilde{\gamma}^*(f) = f$. So the maps $\tilde{\gamma}^*$ and $\tilde{\Sigma}$ are mutually inverse. \square

~ V Induction / Base change

Given a ring map $\phi: \Lambda \rightarrow B$,

We define a "base change" functor which goes in the other direction.

Def¹: Given an Λ -module M and a B -module N , we call an Λ -module map

$u: M \rightarrow \text{res}_{\phi}(N)$ universal if restriction along u provides a bijection

$u^*: \text{Hom}_{B\text{-mod}}(N, N') \rightarrow \text{Hom}_{\Lambda\text{-mod}}(M, \text{res}_{\phi}(N'))$.

$$\alpha^*(g) = \text{res}_g(g) \circ \alpha$$

17

at arbitrary N' in $\mathcal{B}\text{-mod}$.

Equivalently, as it is universal, for each A -module map $w: M \rightarrow \text{res}_g(N')$ w/ generic target there is a uniquely determined \mathcal{B} -module map $f_w: N \rightarrow N'$ which completes a diagram

$$\begin{array}{ccc} & M & \\ \alpha \swarrow & & \searrow w \\ N & \xrightarrow[\exists!]{f_w} & N' \end{array}$$

Proposition 13: Let $\alpha: A \rightarrow B$ be a ring map and M be any A -module.

i) There is a \mathcal{B} -module N which admits a universal A -module map $\alpha: M \rightarrow \text{res}_g(N)$.

ii) For any two universal maps $\alpha_i: M \rightarrow N_i$ there is a unique \mathcal{B} -module isomorphism $f_\alpha: N_0 \rightarrow N_1$ which completes a diagram

$$\begin{array}{ccc} & M & \\ \alpha_0 \swarrow & & \searrow \alpha_1 \\ N_0 & \xrightarrow{f_\alpha} & N_1 \end{array}$$

iii) For any A -module map $\beta: M \rightarrow M'$ and universal maps $\alpha: M \rightarrow \text{res}_g(N)$, $\alpha': M' \rightarrow \text{res}_g(N')$, there is a unique \mathcal{B} -module map $\beta: N \rightarrow N'$ which completes a diagram

$$\begin{array}{ccc} M & \xrightarrow{\beta} & M' \\ \alpha \swarrow & & \searrow \alpha' \\ N & \xrightarrow[\mathcal{B}]{\beta} & N' \end{array}$$

Proof/Construction: (2) Consider the free B -module $B \cdot \{M\} := \bigoplus_{m \in M} B$ on basis M , and let 1_m denote the copy of 1 in the m -th position. For $\text{Univ}_B(M) \subseteq B \cdot \{M\}$ the submodule generated by the relations

$$(*) \quad \begin{cases} 1_{a \cdot m} - \rho(a) 1_m & \text{for } a \text{ in } A \text{ and } m \text{ in } M \\ 1_{m+m'} - 1_m - 1_{m'} & \text{for } m, m' \text{ in } M \end{cases}$$

we define

$$B \otimes_A M := B \cdot \{M\} / \text{Univ}_B(M).$$

For b in B and m in M we take $b \otimes m = \overline{b \cdot 1_m}$ in $B \otimes_A M$, and the relations $(*)$ tell us that the set map $\pi: M \rightarrow B \otimes_A M$, $\pi(m) = 1 \otimes m$, is a map of A -modules from M to $\text{res}_B(B \otimes_A M)$.

Now, for any A -mod map $w: M \rightarrow \text{res}_B N'$ we have the unique B -mod map $f_w: B \cdot \{M\} \rightarrow N'$ w/ $f_w(1_m) = w(m)$, by Lemma 11, and we have f_w vanishing on the relations $(*)$ via A -linearity of w . Hence we obtain a unique B -module map from the quotient $f_w: B \otimes_A M \rightarrow N'$ w/

$$f_w(1 \otimes m) = w(m) \quad \text{at all } b \text{ in } B \text{ and } m \text{ in } M.$$

Further, we observe the existence of a unique B -module map which completes a diagram

$$\begin{array}{ccc} & \mathcal{M} & \\ u \swarrow & & \searrow \omega \\ B \otimes_A \mathcal{M} & \xrightarrow{f_{\omega}} & N \end{array} \quad \text{We're done.}$$

cii) We have the uniquely determined B -module maps $f_{ij}: N_i \rightarrow N_j$, for $i, j \in \{0, 1\}$, which complete the prescribed diagrams. The univ. property then demands

$$f_{ii} = \text{id}_{N_i} \text{ and } f_{jk} \circ f_{ij} = f_{ik} \text{ for each } i, j, k \in \{0, 1\}. \text{ In particular, } f_{01} \circ f_{10} = \text{id}_{N_0} \text{ and } f_{10} \circ f_{01} = \text{id}_{N_1}.$$

ciii) Immediate from the universal property. \square

Def^h: For any A -module \mathcal{M} we let $B \otimes_A \mathcal{M}$ denote any B -module which is equipped with a universal map

$$\eta_{\mathcal{M}}: \mathcal{M} \rightarrow_{\text{res}} B \otimes_A \mathcal{M}.$$

For any map of A -modules $f: \mathcal{M} \rightarrow \mathcal{M}'$ we let $B \otimes_A f: B \otimes_A \mathcal{M} \rightarrow B \otimes_A \mathcal{M}'$ denote the unique B -module map with $(B \otimes_A f) \circ \eta_{\mathcal{M}} = \eta_{\mathcal{M}'} \circ f$.

On generating monomials

$$(B \otimes_A f)(1 \otimes m) = 1 \otimes f(m)$$

$$\text{so that } (B \otimes_A f)(b \otimes m) = b \otimes f(m).$$

Theorem 14: For any map of rings $\phi: A \rightarrow B$,
 there is a functor $\begin{cases} M \mapsto B \otimes_A M \\ f \mapsto B \otimes_A f \end{cases}$
 $B \otimes_A -: A\text{-mod} \rightarrow B\text{-mod}$

Furthermore, the universal maps define a natural transformation:

$$\alpha: \text{id}_{A\text{-mod}} \rightarrow \text{res}_\phi \circ (B \otimes_A -)$$

for which, at each M in $A\text{-mod}$ and N in $B\text{-mod}$,
 the map

$$\text{Hom}_{B\text{-mod}}(B \otimes_A M, N) \longrightarrow \text{Hom}_{A\text{-mod}}(M, \text{res}_\phi(N))$$

$$g \longmapsto \text{res}_\phi(g) \circ \alpha_M$$

is an isomorphism.

Proof: The second assertion just follows by Prop 13
 (iii) and the universal property. We need only check

$$\text{that } B \otimes_A \text{id}_M = \text{id}_{B \otimes_A M} \text{ and } (B \otimes_A g) \circ (B \otimes_A f) = B \otimes_A (g \circ f).$$

The first equality follows by the diagram

$$\begin{array}{ccc} M & \xrightarrow{\text{id}} & M \\ \alpha \downarrow & & \downarrow \alpha \\ B \otimes_A M & \xrightarrow{\text{id}} & B \otimes_A M \end{array}$$

and the second follows by the diag

$$\begin{array}{ccccc} & & & \alpha & \rightarrow M'' \\ & & & \downarrow & \\ M & \xrightarrow{f} & M' & \xrightarrow{g} & M'' \\ \downarrow & \searrow & \downarrow & \searrow & \downarrow \\ B \otimes_A M & \xrightarrow{B \otimes f} & B \otimes_A M' & \xrightarrow{B \otimes g} & B \otimes_A M'' \end{array}$$

6/11

1. Prove that the only ideals in the matrix ring $M_n(k)$, for k a field, are 0 and $M_n(k)$ itself.

2. a) Prove that, for any field k , the standard module $V = k^n$ over $M_n(k)$ is simple. [Hint: Think about row-vec.]

b) Prove that $\text{End}_{M_n(k)}(V) = k \cdot \text{id}_V$. [Hint: Consider eigenvectors for the diagonal matrices, and the action of the super-diagonal.]

3. Classify simple modules over $\mathbb{Q}[x]$.

4. Let k be a commutative ring and A be a k -alg. For a k -module M , prove that the choice of an A -mod structure on M is equivalent to the choice of a k -alg map $\phi: A \rightarrow \text{End}_k(M)$.

5. For any A -module M define the annihilator $\text{Ann}_A(M) \subseteq A$ as the subset of a in A w/ $a \cdot m = 0$ at all m in M . Show that $\text{Ann}_A(M)$ is an ideal in A .

6. For any quotient map $\pi: A \rightarrow A/I$ via an ideal $I \subseteq A$, prove that the restriction functor

$$\text{res}_\pi: A/I\text{-mod} \rightarrow A\text{-mod}$$

is fully faithful. Prove, furthermore, that res_π is an equivalence onto the full subcategory in $A\text{-mod}$ consisting of all modules M with $I \subseteq \text{Ann}_A(M)$.

7. a) For any ideal $I \subseteq A$ and A -module M , prove that $I \cdot M = \{ \alpha \cdot m : \alpha \in I, m \in M \} \subseteq M$ is a submodule in M .

b) Prove that the quotient map $M \rightarrow M/I \cdot M$ induces an isomorphism of A/I -modules

$$A/I \otimes_A M \xrightarrow{\cong} M/I \cdot M.$$